<h1 align=center> 第9周高数作业 </h1>



<h4 align=center>王维 </h4>   

-------

## 9.4  

(2)$z=u^{2}lnv \qquad u = \frac{x}{y} \qquad v = 3x-2y$  
$$
\begin{split}
		\frac{\partial z }{\partial x} &= \frac{\partial z}{\partial u} \cdot \frac{\partial u}{\partial x} + \frac{\partial z}{\partial v} \cdot \frac{\partial v}{\partial x}	\\ 
		&= 2ulnv \cdot \frac{1}{y} + \frac{u^2}{v} \cdot 3 \\
		&= \frac{2x}{y^2}ln(3x-2y) + \frac{3x^2}{y^2(3x-2y)}
	\end{split}
$$

$$
	\begin{split}
		\frac{\partial z}{\partial y} &= \frac{\partial z}{\partial u} \cdot \frac{\partial u}{\partial y} + \frac{\partial z}{\partial v} \cdot \frac{\partial v}{\partial y} \\
		&=2ulnv \cdot \frac{-x}{y^2} + \frac{u^2}{v} \cdot (-2) \\
		&= \frac{2x}{y} \cdot \frac{-x}{y^2}ln(3x-2y) + \frac{-2x^2}{y^2(3x-2y)} \\
		&= \frac{-2x^2}{y^3} \cdot ln(3x-2y) + \frac{-2x^2}{y^2(3x-2y)}
	\end{split}
$$

(7) $z = arctan\frac{x}{y} \qquad x = u + v \qquad y = u - v \qquad$
证: $\frac{\partial z}{\partial u} + \frac{\partial z}{\partial v} = \frac{u-v}{u^2+v^2}$

$$
	\begin{split}
		\frac{\partial z}{\partial u} &= \frac{\partial z}{\partial x} \cdot \frac{\partial x}{\partial u} + \frac{\partial z}{\partial y} \cdot \frac{\partial y}{\partial u} \\
		&= \frac{1}{y(1+(\frac{x}{y})^2)} + \frac{-x}{y^2(1+(\frac{x}{y})^2)} \\
		&= \frac{y-x}{y^2 + x^2}
	\end{split}
$$
$$
	\begin{split}
		\frac{\partial z}{\partial v} &= \frac{\partial z}{\partial x} \cdot \frac{\partial x}{\partial v} + \frac{\partial z}{\partial y} \cdot  \frac{\partial y}{\partial v} \\
		&= \frac{1}{y(1+(\frac{x}{y})^2)} + \frac{-x}{y^2(1+(\frac{x}{y})^2)} \cdot (-1) \\
		&= \frac{y+x}{y^2 + x^2}
	\end{split}
	 
$$
$$
	\begin{split}
		\frac{\partial z}{\partial u} + \frac{\partial z}{\partial v} &= \frac{2y}{x^2+ y^2} \\
		&= \frac{u-v}{u^2+v^2}
	\end{split}
$$

(11) $z = \int(x^2+y^2)$ $\qquad \int$具有二阶导数 $\qquad 求\frac{\partial^2 z}{\partial x^2},\frac{\partial^2 z}{\partial x \partial y}, \frac{\partial^2 z}{\partial y^2}$

$$
	令u = x^2 + y^2 \quad 则 z = \int(u) \\
	\begin{split}
		\frac{\partial u}{\partial x} &= \int'(u) \cdot \frac{\partial u}{\partial x} = 2x\int'(u)
	\end{split}
	\\
	\begin{split}
		\frac{\partial u}{\partial y} &= \int'(u) \cdot \frac{\partial u}{\partial y} = 2y\int'(u)
	\end{split}
	\\ \qquad \qquad 
	\begin{split}
		\frac{\partial^2 z }{\partial x^2} &= 2\int'(u) + 4x^2\int''(u) \\
		 &= 2\int'(x^2+ y^2) + 4x^2\int''(x^2+ y^2) 
	\end{split}
$$
$$
	\begin{split}
		\frac{\partial^2 z}{\partial x \partial y} &= 2x\int''(u) \cdot 2y \\
		&= 4xy\int''(u) \\
		&= 4xy\int''(x^2 + y^2)
	\end{split}
$$
$$
	\begin{split}
		\frac{\partial^2 z }{\partial y^2} &= 2\int'(u) + 4y^2\int''(u) \\
		 &= 2\int'(x^2+ y^2) + 4y^2\int''(x^2+ y^2) 
	\end{split}
$$

## 9.5  

(1) $\sin{y} + e^x - xy^2 = 0$

$$
	Fx = e^x - y^2 \qquad Fy = \cos y - 2xy \\
	\begin{split}
		\frac{dy}{dx} &= -\frac{Fx}{Fy} \\
		&= -\frac{e^x - y^2}{\cos y - 2xy} \qquad (Fy \neq 0)
	\end{split}
$$

(3) $x+2y+z-2\sqrt{xyz} = 0$

$$
	Fx = 1 - \frac{\sqrt{yz}}{\sqrt{x}} \qquad Fy = 2 - \frac{\sqrt{xz}}{\sqrt{y}} \qquad Fz = 1 - \frac{\sqrt{xy}}{\sqrt{z}} \\
	\frac{\partial z}{\partial x} = -\frac{Fx}{Fz} = \frac{yz-\sqrt{xyz}}{\sqrt{xyz}-xy} \qquad (Fz \neq 0) \\
	\frac{\partial z}{\partial y} = -\frac{Fy}{Fz} = \frac{xz-2\sqrt{xyz}}{\sqrt{xyz}-xy} \qquad (Fz \neq 0) \\
$$

(5) $2\sin (x+2y-3z) = x+2y-3z$ $\qquad 证 \frac{\partial z}{\partial x}+\frac{\partial z}{\partial y} = 1$
$ \\ \qquad 原式:  2 \sin(x+2y-3z) -x -2y+3z = 0$
$$
	Fx = 2 \cos (x+2y-3z) - 1 \\
	Fy = 4 \cos (x+2y-3z) - 2 \\
	Fz = -6 \cos (x+2y-3z) + 3 \\
	\frac{\partial z}{\partial x}+ \frac{\partial z}{\partial y} = -\frac{Fx}{Fz}- \frac{Fy}{Fz} = \frac{1}{3} + \frac{2}{3} = 1 \\
	证毕
$$
